code/datatypes/Maps.v
@@ -1,45 +1,21 @@
 Require Import CQE.flatCurry EqNat.
 
-Module cuMin_maps.
-
 Inductive id : Type :=
-  | Id : nat -> id.
-
-Definition total_map (A:Type) := id -> A.
-
-Definition partial_map (A:Type) := total_map (option A).
-
-Definition tmap_empty {A:Type} (v : A) : total_map A :=
-  (fun _ => v).
+| Id : nat -> id.
 
 Definition beq_id id1 id2 :=
   match id1,id2 with Id n1, Id n2 => beq_nat n1 n2 end.
 
-Definition t_update {A:Type} (m : total_map A) (x : id) (v : A) :=
-  fun x' => if beq_id x x' then v else m x'.
+Definition total_map (K V : Type) := K -> V.
 
-Definition emptymap {A:Type} : partial_map A := tmap_empty None.
+Definition partial_map (K V : Type) := total_map K (option V).
 
-Definition update {A:Type} (m : partial_map A) (x : id) (v : A) :=
-  t_update m x (Some v).
+Definition tmap_empty {K V : Type} (v : V) : total_map K V := (fun _ => v).
 
-End cuMin_maps.
+Definition emptymap {K V :Type} : partial_map K V := tmap_empty None.
 
-Module flatCurry_maps. (* Redundant Code... *)
+Definition t_update {K V : Type} (beq : K -> K -> bool) (m : total_map K V) (k : K) (v : V) :=
+  fun k' => if beq k k' then v else m k'.
 
-Definition total_map (A:Type) := VarIndex -> A.
-
-Definition partial_map (A:Type) := total_map (option A).
-
-Definition tmap_empty {A:Type} (v : A) : total_map A :=
-  (fun _ => v).
-
-Definition t_update {A:Type} (m : total_map A) (x : VarIndex) (v : A) :=
-  fun x' => if beq_nat x x' then v else m x'.
-
-Definition emptymap {A:Type} : partial_map A := tmap_empty None.
-
-Definition update {A:Type} (m : partial_map A) (x : VarIndex) (v : A) :=
-  t_update m x (Some v).
-
-End flatCurry_maps.
+Definition update {K V : Type} (beq : K -> K -> bool) (m : partial_map K V) (k : K) (v : V) :=
+  t_update beq m k (Some v).
